@prefix mava: <http://example.org/mava/ontology#> .
@prefix adms: <http://www.w3.org/ns/adms#> .
@prefix dcterms: <http://purl.org/dc/terms/> .
@prefix doap: <http://usefulinc.com/ns/doap#> .
@prefix ebucore: <http://www.ebu.ch/metadata/ontologies/ebucore/ebucore#> ..
@prefix owl: <http://www.w3.org/2002/07/owl#> .
@prefix rdf: <http://www.w3.org/1999/02/22-rdf-syntax-ns#> .
@prefix rdfs: <http://www.w3.org/2000/01/rdf-schema#> .
@prefix sh: <http://www.w3.org/ns/shacl#> .
@prefix skos: <http://www.w3.org/2004/02/skos/core#> .
@prefix tei: <http://www.tei-c.org/ns/1.0/> .
@prefix xsd: <http://www.w3.org/2001/XMLSchema#> .

mava: a owl:Ontology ;
  dcterms:title "MAVA Ontology" ;
  dcterms:author "Stefan Milosavljevic" , "Sabine Maennel" , "Robin Franken";
  dcterms:abstract "An ontology for multimodal audio-visual corpora to allow interoperability and data exchange" ;
  dcterms:description "This ontology provides classes and properties for representing corpora, documents, media resources, time and/or text annotations. It is designed to be a reference point for data exchange across annotation tools in linguistics." ;
  adms:versionNotes "Initial version. Please update with release notes as needed." ;
  dcterms:modified "2025-08-12"^^xsd:date ;
  dcterms:created "2025-08-12"^^xsd:date ;
  dcterms:creator "Swiss Data Science Center" ;
  dcterms:issued "2025-08-12"^^xsd:date ;
  dcterms:license <https://creativecommons.org/licenses/by/4.0/> ;
  dcterms:publisher "ETH Zurich" ;
  dcterms:rightsHolder "ETH Zurich" ;
  owl:versionInfo "0.0.1" ;
  doap:repository <https://github.com/sdsc-ordes/mava-api> ;
  rdfs:label "MAVA Ontology" ;
  rdfs:comment "Ontology for corpora, documents, media resources, time and/or text annotations in linguistics." ;
.

mava:Corpus a rdfs:Class, sh:NodeShape ;
    rdfs:label "Corpus" ;
    rdfs:comment "A collection of documents, media resources, and annotations." ;
    skos:definition "A large and structured set of multimodal data (audio, video and/or text) that is collected and stored for the purpose of linguistic analysis." ;
    rdfs:subClassOf dcterms:Collection ;
    sh:property [sh:path mava:hasDocument ;
                 sh:class mava:Document ] .


mava:hasDocument a rdf:Property ;
    rdfs:label "Has document" ;
    rdfs:domain mava:Corpus ;
    rdfs:range mava:Document ;
    rdfs:subPropertyOf dcterms:hasPart .


mava:Document a rdfs:Class, sh:NodeShape ;
    rdfs:label "Document" ;
    rdfs:comment "A document within a corpus, which can contain media resources and annotations." ;
    skos:definition "A unit of a corpus that can be either an audio, video or text." ;
    rdfs:subClassOf dcterms:Text ;
    rdfs:subClassOf tei:TEI ;
    sh:property [sh:path mava:hasMedia ;
                 sh:class mava:MediaResource] ;
    sh:property [sh:path mava:hasTimeline ;
                 sh:class mava:Timeline] ;
    sh:property [sh:path mava:hasTier ;
                 sh:class mava:AnnotationTier] ;
    sh:property [sh:path mava:documentProfile ;
                 sh:datatype xsd:string ] .

mava:hasMedia a rdf:Property ;
    rdfs:label "Has media resource" ;
    rdfs:domain mava:Document ;
    rdfs:range mava:MediaResource ;
    rdfs:subPropertyOf dcterms:hasPart
    .

mava:MediaResource a rdfs:Class, sh:NodeShape ;
    rdfs:label "Media Resource" ;
    rdfs:comment "A media resource such as audio or video within a document." ;
    rdfs:subClassOf ebucore:MediaResource ;
    sh:property [sh:path mava:hasMediaProfile ;
                 sh:datatype xsd:string ] ;
    sh:property [sh:path mava:hasResourceProxy ;
                 sh:class mava:ResourceProxy]
    .

mava:hasMediaProfile a rdf:Property ;
    rdfs:label "Has media profile" ;
    rdfs:domain mava:MediaResource ;
    rdfs:range xsd:string ;
    rdfs:subPropertyOf dcterms:description
    .

mava:hasResourceProxy a rdf:Property ;
    rdfs:label "Has resource proxy" ;
    rdfs:domain mava:MediaResource ;
    rdfs:range mava:ResourceProxy ;
    rdfs:subPropertyOf dcterms:hasPart
    .

mava:ResourceProxy a rdfs:Class ;
    rdfs:label "Resource Proxy" ;
    rdfs:comment "A proxy for a media resource, which can be used to reference the resource in a different context." ;
    rdfs:subClassOf ebucore:ResourceProxy ;
    .

mava:Timeline a rdfs:Class, sh:NodeShape ;
    rdfs:label "Timeline" ;
    rdfs:comment "A timeline for a document, which can contain annotations." ;
    rdfs:subClassOf tei:Timeline ;
    sh:property [sh:path mava:hasSegment ;
                sh:class mava:Segment] ;
    .

mava:hasSegment a rdf:Property ;
    rdfs:label "Has segment" ;
    rdfs:domain mava:Timeline ;
    rdfs:range mava:Segment ;
    rdfs:subPropertyOf dcterms:hasPart .

mava:Segment a rdfs:Class, sh:NodeShape ;
    rdfs:label "Segment" ;
    rdfs:comment "A segment within a timeline, which can represent a time span or a text span." ;
    skos:definition "Defined portion of audio or video marked by specific start and end times" ;
    rdfs:subClassOf tei:Span ;
    sh:property [sh:path mava:annotatedBy ;
                 sh:class mava:Annotation] ;
    .

mava:annotatedBy a rdf:Property ;
    rdfs:label "Annotated by" ;
    rdfs:domain mava:Segment ;
    rdfs:range mava:Annotation ;
    rdfs:subPropertyOf dcterms:hasPart .

mava:Annotation a rdfs:Class, sh:NodeShape ;
    rdfs:label "Annotation" ;
    rdfs:comment "An annotation for a segment, which can provide additional information or context." ;
    skos:definition "Structured piece of metadata that links specific segments of audio, video, or text to defined concepts or entities." ;
    rdfs:subClassOf tei:Span ;
    sh:property [sh:path mava:linksTo ;
                sh:class mava:Link ] ;
    sh:property [sh:path mava:createdBy ;
                 sh:class mava:Agent ] ;
    .

mava:linksTo a rdf:Property ;
    rdfs:label "Links to" ;
    rdfs:domain mava:Annotation ;
    rdfs:range mava:Link ;
    rdfs:subPropertyOf dcterms:relation .

mava:createdBy a rdf:Property ;
    rdfs:label "Created by" ;
    rdfs:domain mava:Annotation ;
    rdfs:range mava:Agent ;
    rdfs:subPropertyOf dcterms:creator .


mava:Tier a rdfs:Class ;
    rdfs:label "Annotation Tier" ;
    skos:definition "Structured layer of related annotations grouped together to represent a specific linguistic or semantic feature" .


mava:start a rdf:Property ;
    rdfs:label "Start time" ;
    rdfs:subPropertyOf tei:from ;
    rdfs:domain mava:Segment ;
    rdfs:range xsd:string ;
    skos:example "00:01:32" .

mava:end a rdf:Property ;
    rdfs:label "End time" ;
    rdfs:subPropertyOf tei:to ;
    rdfs:domain mava:Segment ;
    rdfs:range xsd:string ;
    skos:example "00:02:45" .

mava:value a rdf:Property ;
    rdfs:label "Annotation value" ;
    rdfs:subPropertyOf tei:content .

mava:belongsToTier a rdf:Property ;
    rdfs:label "Belongs to tier" .

mava:hasTimeline a rdf:Property ;
  rdfs:label "Has timeline" ;
  rdfs:comment "Relates a document to its timeline." .

mava:documentProfile a rdf:Property ;
  rdfs:label "Document profile" ;
  rdfs:comment "A descriptive profile for the document." .

mava:hasTier a rdf:Property ;
  rdfs:label "Has tier" ;
  rdfs:comment "Relates a document to an annotation tier." .
