@prefix adms: <http://www.w3.org/ns/adms#> .
@prefix dcterms: <http://purl.org/dc/terms/> .
@prefix doap: <http://usefulinc.com/ns/doap#> .
@prefix mava: <http://example.org/mava/ontology#> .
@prefix owl: <http://www.w3.org/2002/07/owl#> .
@prefix rdf: <http://www.w3.org/1999/02/22-rdf-syntax-ns#> .
@prefix rdfs: <http://www.w3.org/2000/01/rdf-schema#> .
@prefix xsd: <http://www.w3.org/2001/XMLSchema#> .

mava: a owl:Ontology ;
  dcterms:title "MAVA Ontology" ;
  dcterms:author "Stefan Milosavljevic" , "Sabine Maennel" , "Robin Franken";
  dcterms:abstract "An ontology for multimodal audio-visual corpora to allow interoperability and data exchange" ;
  dcterms:description "This ontology provides classes and properties for representing corpora, documents, media resources, time and/or text annotations. It is designed to be a reference point for data exchange across annotation tools in linguistics." ;
  adms:versionNotes "Initial version. Please update with release notes as needed." ;
  dcterms:modified "2025-08-12"^^xsd:date ;
  dcterms:created "2025-08-12"^^xsd:date ;
  dcterms:creator "Swiss Data Science Center" ;
  dcterms:issued "2025-08-12"^^xsd:date ;
  dcterms:license <https://creativecommons.org/licenses/by/4.0/> ;
  dcterms:publisher "ETH Zurich" ;
  dcterms:rightsHolder "ETH Zurich" ;
  owl:versionInfo "0.0.1" ;
  doap:repository <https://github.com/sdsc-ordes/mava-api> ;
  rdfs:label "MAVA Ontology" ;
  rdfs:comment "Ontology for corpora, documents, media resources, time and/or text annotations in linguistics." ;
.

# --- Core Classes ---

mava:VideoCorpus a owl:Class ;
    rdfs:label "Video Corpus" ;
    rdfs:comment "A collection of videos that share a common context or purpose." ;
    rdfs:subClassOf dcterms:Collection .

mava:Video a owl:Class ;
    rdfs:label "Video" ;
    rdfs:comment "A media resource consisting of a sequence of images creating the illusion of movement." ;
    rdfs:subClassOf dcterms:MovingImage .

mava:AnnotationSeries a owl:Class ;
    rdfs:label "Annotation Series" ;
    rdfs:comment "A series of annotations for a video that align to intervals on its timeline." .

mava:AnnotationSegment a owl:Class ;
    rdfs:label "Annotation Segment" ;
    rdfs:comment "A defined portion of a timeline marked by a specific start and end time with an annotation that relates to that segment of the video." .

mava:ObservationSeries a owl:Class ;
    rdfs:label "Observation Series" ;
    rdfs:comment "A collection of observations at time points in a video." .

mava:ObservationPoint a owl:Class ;
    rdfs:label "Observation Point" ;
    rdfs:comment "A single quantitative value recorded at a specific point on the timeline of a video." .

# --- Properties to Link Videos ---

# Corpus and Video
mava:hasMember a owl:ObjectProperty ;
    rdfs:label "has member" ;
    rdfs:domain mava:VideoCorpus ;
    rdfs:range mava:Video .

mava:hasAnalysis a owl:ObjectProperty ;
    rdfs:label "has analysis" ;
    rdfs:comment "Relates a video to its analysis series." ;
    rdfs:domain mava:Video ;
    rdfs:range mava:ObservationSeries, mava:AnnotationSeries .

# --- Properties to Link Videos Analysis ---

mava:seriesDescription a owl:DatatypeProperty ;
    rdfs:label "series description" ;
    rdfs:domain mava:AnnotationSeries, mava:ObservationSeries ;
    rdfs:range xsd:string .

mava:valueDescription a owl:DatatypeProperty ;
    rdfs:label "value description" ;
    rdfs:domain mava:AnnotationSeries, mava:ObservationSeries ;
    rdfs:range xsd:string .

mava:belongsToAnnotationSeries a owl:ObjectProperty ;
    rdfs:label "belongs to annotation series" ;
    rdfs:comment "Relates a data point back to the data series it is a member of." ;
    rdfs:domain mava:AnnotationSegment ;
    rdfs:range mava:AnnotationSeries .

mava:belongsToObservationSeries a owl:ObjectProperty ;
    rdfs:label "belongs to observation series" ;
    rdfs:comment "Relates a time interval back to the data series it is a member of." ;
    rdfs:domain mava:ObservationPoint ;
    rdfs:range mava:ObservationSeries .

# --- Properties to Link Videos Analysis Times ---

mava:atTime a owl:DatatypeProperty ;
    rdfs:label "at time" ;
    rdfs:domain mava:ObservationPoint;
    rdfs:range xsd:decimal .

mava:startTime a owl:DatatypeProperty ;
    rdfs:label "start time" ;
    rdfs:domain mava:AnnotationSegment ;
    rdfs:range xsd:decimal .

mava:endTime a owl:DatatypeProperty ;
    rdfs:label "end time" ;
    rdfs:domain mava:AnnotationSegment ;
    rdfs:range xsd:decimal .

# --- Properties to Link Videos Analysis Values ---

mava:numericValue a owl:DatatypeProperty ;
    rdfs:label "numeric value" ;
    rdfs:domain mava:ObservationPoint ;
    rdfs:range xsd:decimal .

mava:listValue a owl:DatatypeProperty ;
    rdfs:label "list value" ;
    rdfs:domain mava:ObservationPoint, mava:AnnotationSegment ;
    rdfs:range rdf:List .

mava:stringValue a owl:DatatypeProperty ;
    rdfs:label "string value" ;
    rdfs:domain mava:ObservationPoint, mava:AnnotationSegment ;
    rdfs:range xsd:string .
